proofs/fstar/extraction/Sandwich.Implementation.Openssl3_impl.fsti
@@ -1,0 +1,198 @@
+module Sandwich.Implementation.Openssl3_impl
+#set-options "--fuel 0 --ifuel 1 --z3rlimit 15"
+open Core
+open FStar.Mul
+
+let _ =
+  (* This module has implicit dependencies, here we make them explicit. *)
+  (* The implicit dependencies arise from typeclasses instances. *)
+  let open Sandwich.Error in
+  let open Sandwich.Error.Code in
+  let open Std.Ffi.Os_str in
+  ()
+
+/// The default provider name.
+let v_DEFAULT_PROVIDER_NAME: t_Array u8 (sz 8) =
+  let list = [100uy; 101uy; 102uy; 97uy; 117uy; 108uy; 116uy; 0uy] in
+  FStar.Pervasives.assert_norm (Prims.eq2 (List.Tot.length list) 8);
+  Rust_primitives.Hax.array_of_list 8 list
+
+/// Pointer to the default provider name.
+let v_DEFAULT_PROVIDER_NAME_PTR: Rust_primitives.Hax.t_failure =
+  Rust_primitives.Hax.failure "(reject_RawOrMutPointer) ExplicitRejection { reason: \"a node of kind [Raw_pointer] have been found in the AST\" }"
+    "core::ptr::const_ptr::impl__cast::<\n        int,\n        int,\n    >(\n        rust_primitives::hax::failure(\n            \"(AST import) something is not implemented yet.\\nPointer, with [cast] being Types.ArrayToPointer\",\n            \"{ Types.attributes = [];\\n  contents =\\n  Types.PointerCoercion {cast = Types.ArrayToPointer;\\n    source =\\n    { Types.attributes = [];\\n      contents =\\n      Types.AddressOf {\\n        arg =\\n        { Types.attributes = [];\\n          contents =\\n          Types.Deref {\\n            arg =\\n            { Types.attributes = [];\\n              contents =\\n              Types.NamedConst {args = [];\\n                def_id =\\n                { Types.index = (0, 511); krate = \\\"sandwich\\\";\\n                  path =\\n                  [{ Types.data = (Types.TypeNs \\\"implementation\\\");\\n                     disambiguator = 0 };\\n                    { Types.data = (Types.TypeNs \\\"openssl3_impl\\\");\\n                      disambiguator = 0 };\\n                    { Types.data = (Types.ValueNs \\\"DEFAULT_PROVIDER_NAME\\\");\\n                      disambiguator = 0 }\\n                    ]\\n                  };\\n                impl = None; user_ty = None};\\n              hir_id = None;\\n              span =\\n              { Types.filename =\\n                (Types.Real\\n                   (Types.LocalPath\\n                      \\\"rust/implementation/openssl3_impl/mod.rs\\\"));\\n                hi = { Types.col = \\\"71\\\"; line = \\\"29\\\" };\\n                lo = { Types.col = \\\"50\\\"; line = \\\"29\\\" } };\\n              ty =\\n              (Types.Ref\\n                 ({ Types.kind = Types.ReErased },\\n                  (Types.Array\\n                     ((Types.Uint Types.U8),\\n                      { Types.attributes = [];\\n                        contents =\\n                        (Types.Literal\\n                           (Types.Int (Types.Uint (\\\"8\\\", Types.Usize))));\\n                        hir_id = None;\\n                        span =\\n                        { Types.filename =\\n                          (Types.Real (Types.LocalPath \\\"rust/lib.rs\\\"));\\n                          hi = { Types.col = \\\"0\\\"; line = \\\"1\\\" };\\n                          lo = { Types.col = \\\"0\\\"; line = \\\"1\\\" } };\\n                        ty = (Types.Uint Types.Usize) })),\\n                  false))\\n              }};\\n          hir_id = None;\\n          span =\\n          { Types.filename =\\n            (Types.Real\\n               (Types.LocalPath \\\"rust/implementation/openssl3_impl/mod.rs\\\"));\\n            hi = { Types.col = \\\"71\\\"; line = \\\"29\\\" };\\n            lo = { Types.col = \\\"50\\\"; line = \\\"29\\\" } };\\n          ty =\\n          (Types.Array\\n             ((Types.Uint Types.U8),\\n              { Types.attributes = [];\\n                contents =\\n                (Types.Literal (Types.Int (Types.Uint (\\\"8\\\", Types.Usize))));\\n                hir_id = None;\\n                span =\\n                { Types.filename =\\n                  (Types.Real (Types.LocalPath \\\"rust/lib.rs\\\"));\\n                  hi = { Types.col = \\\"0\\\"; line = \\\"1\\\" };\\n                  lo = { Types.col = \\\"0\\\"; line = \\\"1\\\" } };\\n                ty = (Types.Uint Types.Usize) }))\\n          };\\n        mutability = false};\\n      hir_id = (Some (\\\"513\\\", \\\"7\\\"));\\n      span =\\n      { Types.filename =\\n        (Types.Real\\n           (Types.LocalPath \\\"rust/implementation/openssl3_impl/mod.rs\\\"));\\n        hi = { Types.col = \\\"71\\\"; line = \\\"29\\\" };\\n        lo = { Types.col = \\\"50\\\"; line = \\\"29\\\" } };\\n      ty =\\n      (Types.RawPtr\\n         ((Types.Array\\n             ((Types.Uint Types.U8),\\n              { Types.attributes = [];\\n                contents =\\n                (Types.Literal (Types.Int (Types.Uint (\\\"8\\\", Types.Usize))));\\n                hir_id = None;\\n                span =\\n                { Types.filename =\\n                  (Types.Real (Types.LocalPath \\\"rust/lib.rs\\\"));\\n                  hi = { Types.col = \\\"0\\\"; line = \\\"1\\\" };\\n                  lo = { Types.col = \\\"0\\\"; line = \\\"1\\\" } };\\n                ty = (Types.Uint Types.Usize) })),\\n          false))\\n      }};\\n  hir_id = (Some (\\\"513\\\", \\\"6\\\"));\\n  span =\\n  { Types.filename =\\n    (Types.Real (Types.LocalPath \\\"rust/implementation/openssl3_impl/mod.rs\\\"));\\n    hi = { Types.col = \\\"85\\\"; line = \\\"29\\\" };\\n    lo = { Types.col = \\\"49\\\"; line = \\\"29\\\" } };\\n  ty = (Types.RawPtr ((Types.Uint Types.U8), false)) }\",\n        ),\n    )"
+
+/// The oqs-provider provider name.
+let v_OQS_PROVIDER_NAME: t_Array u8 (sz 12) =
+  let list = [111uy; 113uy; 115uy; 112uy; 114uy; 111uy; 118uy; 105uy; 100uy; 101uy; 114uy; 0uy] in
+  FStar.Pervasives.assert_norm (Prims.eq2 (List.Tot.length list) 12);
+  Rust_primitives.Hax.array_of_list 12 list
+
+/// Pointer to the oqs-provider provider name.
+let v_OQS_PROVIDER_NAME_PTR: Rust_primitives.Hax.t_failure =
+  Rust_primitives.Hax.failure "(reject_RawOrMutPointer) ExplicitRejection { reason: \"a node of kind [Raw_pointer] have been found in the AST\" }"
+    "core::ptr::const_ptr::impl__cast::<\n        int,\n        int,\n    >(\n        rust_primitives::hax::failure(\n            \"(AST import) something is not implemented yet.\\nPointer, with [cast] being Types.ArrayToPointer\",\n            \"{ Types.attributes = [];\\n  contents =\\n  Types.PointerCoercion {cast = Types.ArrayToPointer;\\n    source =\\n    { Types.attributes = [];\\n      contents =\\n      Types.AddressOf {\\n        arg =\\n        { Types.attributes = [];\\n          contents =\\n          Types.Deref {\\n            arg =\\n            { Types.attributes = [];\\n              contents =\\n              Types.NamedConst {args = [];\\n                def_id =\\n                { Types.index = (0, 514); krate = \\\"sandwich\\\";\\n                  path =\\n                  [{ Types.data = (Types.TypeNs \\\"implementation\\\");\\n                     disambiguator = 0 };\\n                    { Types.data = (Types.TypeNs \\\"openssl3_impl\\\");\\n                      disambiguator = 0 };\\n                    { Types.data = (Types.ValueNs \\\"OQS_PROVIDER_NAME\\\");\\n                      disambiguator = 0 }\\n                    ]\\n                  };\\n                impl = None; user_ty = None};\\n              hir_id = None;\\n              span =\\n              { Types.filename =\\n                (Types.Real\\n                   (Types.LocalPath\\n                      \\\"rust/implementation/openssl3_impl/mod.rs\\\"));\\n                hi = { Types.col = \\\"63\\\"; line = \\\"35\\\" };\\n                lo = { Types.col = \\\"46\\\"; line = \\\"35\\\" } };\\n              ty =\\n              (Types.Ref\\n                 ({ Types.kind = Types.ReErased },\\n                  (Types.Array\\n                     ((Types.Uint Types.U8),\\n                      { Types.attributes = [];\\n                        contents =\\n                        (Types.Literal\\n                           (Types.Int (Types.Uint (\\\"12\\\", Types.Usize))));\\n                        hir_id = None;\\n                        span =\\n                        { Types.filename =\\n                          (Types.Real (Types.LocalPath \\\"rust/lib.rs\\\"));\\n                          hi = { Types.col = \\\"0\\\"; line = \\\"1\\\" };\\n                          lo = { Types.col = \\\"0\\\"; line = \\\"1\\\" } };\\n                        ty = (Types.Uint Types.Usize) })),\\n                  false))\\n              }};\\n          hir_id = None;\\n          span =\\n          { Types.filename =\\n            (Types.Real\\n               (Types.LocalPath \\\"rust/implementation/openssl3_impl/mod.rs\\\"));\\n            hi = { Types.col = \\\"63\\\"; line = \\\"35\\\" };\\n            lo = { Types.col = \\\"46\\\"; line = \\\"35\\\" } };\\n          ty =\\n          (Types.Array\\n             ((Types.Uint Types.U8),\\n              { Types.attributes = [];\\n                contents =\\n                (Types.Literal (Types.Int (Types.Uint (\\\"12\\\", Types.Usize))));\\n                hir_id = None;\\n                span =\\n                { Types.filename =\\n                  (Types.Real (Types.LocalPath \\\"rust/lib.rs\\\"));\\n                  hi = { Types.col = \\\"0\\\"; line = \\\"1\\\" };\\n                  lo = { Types.col = \\\"0\\\"; line = \\\"1\\\" } };\\n                ty = (Types.Uint Types.Usize) }))\\n          };\\n        mutability = false};\\n      hir_id = (Some (\\\"516\\\", \\\"7\\\"));\\n      span =\\n      { Types.filename =\\n        (Types.Real\\n           (Types.LocalPath \\\"rust/implementation/openssl3_impl/mod.rs\\\"));\\n        hi = { Types.col = \\\"63\\\"; line = \\\"35\\\" };\\n        lo = { Types.col = \\\"46\\\"; line = \\\"35\\\" } };\\n      ty =\\n      (Types.RawPtr\\n         ((Types.Array\\n             ((Types.Uint Types.U8),\\n              { Types.attributes = [];\\n                contents =\\n                (Types.Literal (Types.Int (Types.Uint (\\\"12\\\", Types.Usize))));\\n                hir_id = None;\\n                span =\\n                { Types.filename =\\n                  (Types.Real (Types.LocalPath \\\"rust/lib.rs\\\"));\\n                  hi = { Types.col = \\\"0\\\"; line = \\\"1\\\" };\\n                  lo = { Types.col = \\\"0\\\"; line = \\\"1\\\" } };\\n                ty = (Types.Uint Types.Usize) })),\\n          false))\\n      }};\\n  hir_id = (Some (\\\"516\\\", \\\"6\\\"));\\n  span =\\n  { Types.filename =\\n    (Types.Real (Types.LocalPath \\\"rust/implementation/openssl3_impl/mod.rs\\\"));\\n    hi = { Types.col = \\\"77\\\"; line = \\\"35\\\" };\\n    lo = { Types.col = \\\"45\\\"; line = \\\"35\\\" } };\\n  ty = (Types.RawPtr ((Types.Uint Types.U8), false)) }\",\n        ),\n    )"
+
+(* item error backend: (reject_RawOrMutPointer) ExplicitRejection { reason: "a node of kind [Raw_pointer] have been found in the AST" }
+Last available AST for this item:
+
+/// A convenient builder for providers.
+#[cfg(feature = "openssl3")]
+#[deny(bare_trait_objects)]
+#[feature(register_tool)]
+#[register_tool(_hax)]
+struct t_ProviderBuilder {
+    /// Name of the provider, C format.
+    f_name: core::option::t_Option<raw_pointer!()>,
+    /// Library context.
+    f_lib_ctx: core::option::t_Option<
+        core::ptr::non_null::t_NonNull<openssl3::t_ossl_lib_ctx_st>,
+    >,
+}
+
+
+Last AST:
+/** print_rust: pitem: not implemented  (item: { Concrete_ident.T.def_id =
+  { Concrete_ident.Imported.krate = "sandwich";
+    path =
+    [{ Concrete_ident.Imported.data =
+       (Concrete_ident.Imported.TypeNs "implementation"); disambiguator = 0 };
+      { Concrete_ident.Imported.data =
+        (Concrete_ident.Imported.TypeNs "openssl3_impl"); disambiguator = 0 };
+      { Concrete_ident.Imported.data =
+        (Concrete_ident.Imported.TypeNs "ProviderBuilder"); disambiguator = 0
+        }
+      ]
+    };
+  kind = Concrete_ident.Kind.Value }) */
+const _: () = ();
+ *)
+
+/// Sets the library context.
+val impl__ProviderBuilder__lib_ctx
+      (self: t_ProviderBuilder)
+      (lib_ctx: Core.Ptr.Non_null.t_NonNull Openssl3.t_ossl_lib_ctx_st)
+    : Prims.Pure t_ProviderBuilder Prims.l_True (fun _ -> Prims.l_True)
+
+(* item error backend: (reject_RawOrMutPointer) ExplicitRejection { reason: "a node of kind [Raw_pointer] have been found in the AST" }
+Last available AST for this item:
+
+/// Sets the name.
+#[cfg(feature = "openssl3")]
+#[deny(bare_trait_objects)]
+#[feature(register_tool)]
+#[register_tool(_hax)]
+fn impl__ProviderBuilder__name(
+    self: sandwich::implementation::openssl3_impl::t_ProviderBuilder,
+    name: raw_pointer!(),
+) -> sandwich::implementation::openssl3_impl::t_ProviderBuilder {
+    {
+        sandwich::implementation::openssl3_impl::ProviderBuilder {
+            f_name: core::option::Option_Some(name),
+            ..(self)
+        }
+    }
+}
+
+
+Last AST:
+/** print_rust: pitem: not implemented  (item: { Concrete_ident.T.def_id =
+  { Concrete_ident.Imported.krate = "sandwich";
+    path =
+    [{ Concrete_ident.Imported.data =
+       (Concrete_ident.Imported.TypeNs "implementation"); disambiguator = 0 };
+      { Concrete_ident.Imported.data =
+        (Concrete_ident.Imported.TypeNs "openssl3_impl"); disambiguator = 0 };
+      { Concrete_ident.Imported.data = Concrete_ident.Imported.Impl;
+        disambiguator = 2 };
+      { Concrete_ident.Imported.data =
+        (Concrete_ident.Imported.ValueNs "name"); disambiguator = 0 }
+      ]
+    };
+  kind = Concrete_ident.Kind.Value }) */
+const _: () = ();
+ *)
+
+/// Initializes a builder.
+val impl__ProviderBuilder__new: Prims.unit
+  -> Prims.Pure t_ProviderBuilder Prims.l_True (fun _ -> Prims.l_True)
+
+[@@ FStar.Tactics.Typeclasses.tcinstance]
+let impl_1: Core.Default.t_Default t_ProviderBuilder =
+  {
+    f_default_pre = (fun (_: Prims.unit) -> true);
+    f_default_post = (fun (_: Prims.unit) (out: t_ProviderBuilder) -> true);
+    f_default = fun (_: Prims.unit) -> impl__ProviderBuilder__new ()
+  }
+
+/// A wrapper around an `OSSL_PROVIDER`.
+type t_Provider =
+  | Provider : Sandwich.Support.Pimpl.t_Pimpl Openssl3.t_ossl_provider_st -> t_Provider
+
+[@@ FStar.Tactics.Typeclasses.tcinstance]
+let impl: Core.Fmt.t_Debug t_Provider =
+  {
+    f_fmt_pre = (fun (self: t_Provider) (f: Core.Fmt.t_Formatter) -> true);
+    f_fmt_post
+    =
+    (fun
+        (self: t_Provider)
+        (f: Core.Fmt.t_Formatter)
+        (out1: (Core.Fmt.t_Formatter & Core.Result.t_Result Prims.unit Core.Fmt.t_Error))
+        ->
+        true);
+    f_fmt
+    =
+    fun (self: t_Provider) (f: Core.Fmt.t_Formatter) ->
+      let tmp0, out:(Core.Fmt.t_Formatter & Core.Result.t_Result Prims.unit Core.Fmt.t_Error) =
+        Core.Fmt.impl_7__write_fmt f
+          (Core.Fmt.impl_2__new_v1 (sz 1)
+              (sz 1)
+              (let list = ["Provider("] in
+                FStar.Pervasives.assert_norm (Prims.eq2 (List.Tot.length list) 1);
+                Rust_primitives.Hax.array_of_list 1 list)
+              (let list =
+                  [
+                    Rust_primitives.Hax.failure "(reject_RawOrMutPointer) ExplicitRejection { reason: \"a node of kind [Raw_pointer] have been found in the AST\" }"
+                      "core::fmt::rt::impl_1__new_pointer::<\n        lifetime!(something),\n        raw_pointer!(),\n    >(\n        &(deref(\n            &(core::ptr::non_null::impl_3__as_ptr::<\n                openssl3::t_ossl_provider_st,\n            >(\n                sandwich::support::pimpl::impl_2__as_nonnull::<\n                    lifetime!(something),\n                    openssl3::t_ossl_provider_st,\n                >(&(proj_sandwich::implementation::openssl3_impl::_0(deref(self)))),\n            )),\n        )),\n    )"
+
+                    <:
+                    Core.Fmt.Rt.t_Argument
+                  ]
+                in
+                FStar.Pervasives.assert_norm (Prims.eq2 (List.Tot.length list) 1);
+                Rust_primitives.Hax.array_of_list 1 list)
+            <:
+            Core.Fmt.t_Arguments)
+      in
+      let f:Core.Fmt.t_Formatter = tmp0 in
+      let hax_temp_output:Core.Result.t_Result Prims.unit Core.Fmt.t_Error = out in
+      f, hax_temp_output
+      <:
+      (Core.Fmt.t_Formatter & Core.Result.t_Result Prims.unit Core.Fmt.t_Error)
+  }
+
+/// Builds the provider.
+val impl__ProviderBuilder__build (self: t_ProviderBuilder)
+    : Prims.Pure (Core.Result.t_Result t_Provider Sandwich.Error.t_Error)
+      Prims.l_True
+      (fun _ -> Prims.l_True)
+
+/// An `OSSL_LIB_CTX` object wrapped in a `Pimpl`.
+type t_LibCtx = {
+  f__oqs_provider:t_Provider;
+  f__default_provider:t_Provider;
+  f_lib_ctx:Sandwich.Support.Pimpl.t_Pimpl Openssl3.t_ossl_lib_ctx_st
+}
+
+/// Returns a pointer to the top-level library context.
+val impl_3__as_nonnull (self: t_LibCtx)
+    : Prims.Pure (Core.Ptr.Non_null.t_NonNull Openssl3.t_ossl_lib_ctx_st)
+      Prims.l_True
+      (fun _ -> Prims.l_True)
+
+/// Instantiates a new top-level library context.
+val impl_3__try_new: Prims.unit
+  -> Prims.Pure (Core.Result.t_Result t_LibCtx Sandwich.Error.t_Error)
+      Prims.l_True
+      (fun _ -> Prims.l_True)
